src/program_proof/ctrexample/client.v
@@ -1,7 +1,6 @@
 From Perennial.goose_lang Require Import prelude.
 From Perennial.goose_lang Require Export ffi.grove_prelude.
 From Perennial.program_proof Require Import proof_prelude.
-From Perennial.goose_lang Require Export ffi.grove_filesys_axioms.
 From Perennial.program_proof.ctrexample Require Import interface.
 From Perennial.program_proof Require Import marshal_proof.
 From Goose.github_com.mit_pdos.gokv.ctrexample Require Import client.
